various nits in Key

secure_api/box/functor_box/Box.Key.fst
@@ -10,10 +10,10 @@ open FStar.HyperStack
 open FStar.HyperStack.ST
 open Crypto.Symmetric.Bytes
 
-open Box.Index
-open Box.Plain
 open Box.Flags
 
+module ID = Box.Index
+module Plain = Box.Plain
 module MR = FStar.Monotonic.RRef
 module HH = FStar.HyperHeap
 module HS = FStar.HyperStack
@@ -22,9 +22,12 @@ module SPEC = Spec.SecretBox
 
 assume val is_random: bytes -> Type0
 
-type log_region (im:index_module) =
-  r:MR.rid{disjoint r (get_rgn im)}
+let index_module = ID.index_module
+let plain_module = Plain.plain_module
+let id = ID.id
 
+type log_region =
+  r:MR.rid{is_eternal_region r}
 
 type key_t (im:index_module) (pm:plain_module)= Type0
 
@@ -36,29 +39,29 @@ type key_t (im:index_module) (pm:plain_module)= Type0
 abstract noeq type key_module (im:index_module) =
   | KM:
     keylen: nat ->
-    key_type: (kim:index_module{kim == im} -> t:Type0) ->
+    key_type: (im':index_module{im' == im} -> t:Type0) ->
     get_index: (k:key_type im -> i:id im) -> // You have to have faith in this function...
     get_rawGT: ((k:key_type im) -> GTot (b:lbytes keylen)) -> // You have to have faith in this function...
     invariant: (h:mem -> Type0) ->
-    key_log_region: (log_region im) ->
+    key_log_region: (rgn:log_region{disjoint rgn (ID.get_rgn im)}) ->
     gen: (i:id im -> ST (k:key_type im{get_index k = i}) // The spec should indicate that the result is random and that gen is idempotent
       (requires (fun h0 ->
-        (fresh im i h0 \/ honest im i)
+        (ID.fresh im i h0 \/ ID.honest im i)
         /\ invariant h0))
       (ensures  (fun h0 k h1 ->
         invariant h1
         /\ modifies (Set.singleton key_log_region) h0 h1
         ))) ->
     set: ((i:id im {Game3? current_game \/ Game0? current_game}) -> (b:lbytes keylen) -> (k:key_type im{get_index k = i /\ b = get_rawGT k})) ->
-    coerce: (i:id im{dishonest im i} -> raw:lbytes keylen -> (k:key_type im{get_index k = i /\ raw=get_rawGT k})) ->
-    leak: (k:key_type im{dishonest im (get_index k)} -> (raw:lbytes keylen{raw = get_rawGT k})) ->
+    coerce: (i:id im{ID.dishonest im i} -> raw:lbytes keylen -> (k:key_type im{get_index k = i /\ raw=get_rawGT k})) ->
+    leak: (k:key_type im{ID.dishonest im (get_index k)} -> (raw:lbytes keylen{raw = get_rawGT k})) ->
     key_module im
 
-val get_keylen: im:index_module -> km:key_module im -> nat
+val get_keylen: im:index_module -> km:key_module im -> n:nat{n = km.keylen}
 let get_keylen im km =
   km.keylen
 
-val get_keytype: im:index_module -> km:key_module im -> Type0
+val get_keytype: im:index_module -> km:key_module im -> t:Type0{t == km.key_type im}
 let get_keytype im km =
   km.key_type im
 
@@ -70,13 +73,13 @@ val get_rawGT: im:index_module -> km:key_module im -> gr:(k:km.key_type im -> GT
 let get_rawGT im km =
   km.get_rawGT
 
-val get_log_region: im:index_module -> km:key_module im -> log_region im
+val get_log_region: im:index_module -> km:key_module im -> rgn:log_region{rgn = km.key_log_region}
 let get_log_region im km =
   km.key_log_region
 
 val gen: (im:index_module) -> (km:key_module im) -> (i:id im) -> ST (k:km.key_type im{km.get_index k = i})
   (requires (fun h0 ->
-    (fresh im i h0 \/ honest im i)
+    (ID.fresh im i h0 \/ ID.honest im i)
     /\ km.invariant h0))
   (ensures  (fun h0 k h1 ->
     km.invariant h1
@@ -89,11 +92,11 @@ val set: (im:index_module) -> (km:key_module im) -> (i:id im {Game3? current_gam
 let set im km i b =
   km.set i b
 
-val coerce: (im:index_module) -> (km:key_module im) -> (i:id im{dishonest im i}) -> (b:lbytes km.keylen) -> (k:km.key_type im{km.get_index k = i /\ b = km.get_rawGT k})
+val coerce: (im:index_module) -> (km:key_module im) -> (i:id im{ID.dishonest im i}) -> (b:lbytes km.keylen) -> (k:km.key_type im{km.get_index k = i /\ b = km.get_rawGT k})
 let coerce im km i b =
   km.coerce i b
 
-val leak: im:index_module -> (km:key_module im) -> (k:km.key_type im{dishonest im (km.get_index k)}) -> (b:lbytes km.keylen{b=km.get_rawGT k})
+val leak: im:index_module -> (km:key_module im) -> (k:km.key_type im{ID.dishonest im (km.get_index k)}) -> (b:lbytes km.keylen{b=km.get_rawGT k})
 let leak im km k =
   km.leak k
 
@@ -104,24 +107,25 @@ let invariant im km =
 #set-options "--z3rlimit 2000 --max_ifuel 2 --max_fuel 0"
 val create: (im:index_module) ->
             (keylen: nat) ->
-            (km_key_type: (kim:index_module{kim == im} -> t:Type0)) ->
+            (km_key_type: (im':index_module{im' == im} -> t:Type0)) ->
             (km_get_index: (k:km_key_type im -> i:id im)) -> // You have to have faith in this function...
             (km_get_rawGT: ((k:km_key_type im) -> GTot (b:lbytes keylen))) -> // You have to have faith in this function...
             (km_invariant: (h:mem -> Type0)) ->
-            (km_key_log_region: (log_region im)) ->
+            (km_key_log_region: (r:log_region{disjoint r (ID.get_rgn im)})) ->
             (km_gen: (i:id im -> ST (k:km_key_type im{km_get_index k = i}) // The spec should indicate that the result is random and that gen is idempotent
               (requires (fun h0 ->
-                (fresh im i h0 \/ honest im i)
+                (ID.fresh im i h0 \/ ID.honest im i)
                 /\ km_invariant h0))
               (ensures  (fun h0 k h1 ->
                 km_invariant h1
                 /\ modifies (Set.singleton km_key_log_region) h0 h1
               )))) ->
             (km_set: (i:id im {Game3? current_game \/ Game0? current_game} -> b:lbytes keylen -> (k:km_key_type im{km_get_index k = i /\ b = km_get_rawGT k}))) ->
-            (km_coerce: (i:id im{dishonest im i} -> raw:lbytes keylen -> (k:km_key_type im{km_get_index k = i /\ raw=km_get_rawGT k}))) ->
-            (km_leak: (k:km_key_type im{dishonest im (km_get_index k)} -> (raw:lbytes keylen{raw = km_get_rawGT k}))) ->
+            (km_coerce: (i:id im{ID.dishonest im i} -> raw:lbytes keylen -> (k:km_key_type im{km_get_index k = i /\ raw=km_get_rawGT k}))) ->
+            (km_leak: (k:km_key_type im{ID.dishonest im (km_get_index k)} -> (raw:lbytes keylen{raw = km_get_rawGT k}))) ->
             (km:key_module im{
               get_keytype im km == km_key_type im
+              /\ get_keylen im km == keylen
               /\ get_index im km == km_get_index
               /\ get_rawGT im km == km_get_rawGT
               /\ invariant im km == km_invariant
